@prefix pma: <http://parliament.uk/ontologies/making-available/> . 
@prefix xsd: <http://www.w3.org/2001/XMLSchema#> . 
@prefix rdf: <http://www.w3.org/1999/02/22-rdf-syntax-ns#> .
@prefix dcterms: <http://purl.org/dc/terms/> .
@prefix owl:     <http://www.w3.org/2002/07/owl#> .
@prefix rdfs:    <http://www.w3.org/2000/01/rdf-schema#> .
@prefix foaf:	<http://xmlns.com/foaf/0.1/> .

<http://parliament.uk/ontologies/making-available/> 
    rdf:type owl:Ontology ;
    dcterms:title "Making available ontology"@en ;
    dcterms:created "2018-12-09"^^xsd:date ;
	dcterms:rights "Open Parliament Licence v3.0"@en ;
    dcterms:description "An ontology describing the methods of making materials available to a House or to a House by means of its library."@en;
	foaf:depiction <https://ukparliament.github.io/ontologies/making-available/making-available.png> ;
	foaf:maker
		[ foaf:name "Robert Brook"; foaf:homepage <https://robert-brook.com/> ],
		[ foaf:name "Jack Dent" ],
		[ foaf:name "Michael Smethurst"; foaf:homepage <http://smethur.st/> ],
	    [ foaf:name "Anya Somerville" ].


#######  Classes #####

pma:House rdf:type owl:Class ;
	rdfs:label "House"@en ;
	rdfs:comment "A parliamentary House. For example, the House of Lords."@en ;
	rdfs:isDefinedBy <http://parliament.uk/ontologies/making-available/> .
	
pma:Session rdf:type owl:Class ;
	rdfs:label "Session"@en ;
	rdfs:comment "The period during which Parliament is convened. The first session of a parliament begins on the same day as the parliament period: this date is given in the dissolution proclamation at the end of the previous parliament. The session ends on the day given in a subsequent prorogation proclamation. Subsequent sessions within the parliament begin and end on dates given in prorogation proclamations. The last session of a parliament ends with prorogation followed by dissolution. A session typically lasts for one year. Session periods are the same across both Houses."@en ;
	rdfs:isDefinedBy <http://parliament.uk/ontologies/making-available/> .
	
pma:MakingAvailable rdf:type owl:Class ;
	rdfs:label "Making available"@en ;
	rdfs:comment "The act of making materials available to a House or to a House by means of its library."@en ;
	rdfs:isDefinedBy <http://parliament.uk/ontologies/making-available/> .
	
pma:Laying rdf:type owl:Class ;
	rdfs:subClassOf pma:MakingAvailable ;
	rdfs:label "Laying"@en ;
	rdfs:comment "The act of presenting a paper and supporting documents into either House. Papers may be laid in both Houses on the same day."@en ;
	rdfs:isDefinedBy <http://parliament.uk/ontologies/making-available/> .
	
pma:Depositing rdf:type owl:Class ;
	rdfs:subClassOf pma:MakingAvailable ;
	rdfs:label "Depositing"@en ;
	rdfs:comment "The act of depositing materials into the library of a House."@en ;
	rdfs:isDefinedBy <http://parliament.uk/ontologies/making-available/> .
	
pma:Presenting rdf:type owl:Class ;
	rdfs:subClassOf pma:MakingAvailable ;
	rdfs:label "Presenting"@en ;
	rdfs:comment "The act of presenting materials to a House."@en ;
	rdfs:isDefinedBy <http://parliament.uk/ontologies/making-available/> .
	
	

#######  Object properties ##### 

pma:toHouse rdf:type owl:ObjectProperty ;
	rdfs:label "To House"@en ;
	rdfs:comment "Relates an act of making materials available to a House, to the House in which they are made available."@en ;
	rdfs:domain pma:MakingAvailable ;
	rdfs:range pma:House ;
	rdfs:isDefinedBy <http://parliament.uk/ontologies/making-available/> .
	
pma:inSession rdf:type owl:ObjectProperty ;
	rdfs:label "In session"@en ;
	rdfs:comment "Relates an act of making materials available to a House, to the session in which they are made available."@en ;
	rdfs:domain pma:MakingAvailable ;
	rdfs:range pma:Session ;
	rdfs:isDefinedBy <http://parliament.uk/ontologies/making-available/> .
				

#######  Data properties ##### 

pma:madeAvailableOn rdf:type owl:DatatypeProperty ;
	rdfs:label "Made available on"@en ;
	rdfs:comment "Relates an act of making materials available to a House, to the date on which they are made available."@en ;
	rdfs:domain pma:MakingAvailable ;
	rdfs:range xsd:date ;
	rdfs:isDefinedBy <http://parliament.uk/ontologies/making-available/> .