@prefix pa: <http://parliament.uk/ontologies/agency/> . 
@prefix xsd: <http://www.w3.org/2001/XMLSchema#> . 
@prefix rdf: <http://www.w3.org/1999/02/22-rdf-syntax-ns#> .
@prefix dcterms: <http://purl.org/dc/terms/> .
@prefix owl:     <http://www.w3.org/2002/07/owl#> .
@prefix rdfs:    <http://www.w3.org/2000/01/rdf-schema#> .
@prefix skos: <http://www.w3.org/2004/02/skos/core#> .
@prefix foaf:	<http://xmlns.com/foaf/0.1/> .

<http://parliament.uk/ontologies/agency/> 
    rdf:type owl:Ontology ;
    dcterms:title "Agency ontology"@en ;
    dcterms:created "2016-10-05"^^xsd:date ;
	dcterms:rights "Open Parliament Licence v3.0"@en ;
    dcterms:description "An ontology supporting the description of people and groups by the UK Parliament."@en ;
	foaf:depiction <https://ukparliament.github.io/ontologies/agency/agency.png> ;
	foaf:maker
		[ foaf:name "Robert Brook"; foaf:homepage <https://robert-brook.com/> ],
		[ foaf:name "Silver Oliver" ],
		[ foaf:name "Michael Smethurst"; foaf:homepage <http://smethur.st/> ],
	    [ foaf:name "Anya Somerville" ].


#######  Classes ##### 	

pa:Agent rdf:type owl:Class ;
	rdfs:label "Agent"@en ;
	rdfs:comment "Agents include people and groups, including those outside the Parliamentary Service, participating in parliamentary procedure and contributing to the wider work of Parliament."@en ;
	rdfs:isDefinedBy <http://parliament.uk/ontologies/agency/> .

pa:Person rdf:type owl:Class ;
	rdfs:subClassOf pa:Agent ;
	rdfs:label "Person"@en ;
	rdfs:comment "A person."@en ;
	rdfs:isDefinedBy <http://parliament.uk/ontologies/agency/> .
	
pa:Group rdf:type owl:Class ;
	rdfs:subClassOf pa:Agent ;
	rdfs:label "Group"@en ;
	rdfs:comment "A group of people. Groups may contain other groups or be empty."@en ;
	rdfs:isDefinedBy <http://parliament.uk/ontologies/agency/> .
	
pa:Incumbency rdf:type owl:Class ;
	rdfs:label "Incumbency"@en ;
	rdfs:comment "The holding of a position by a person, including the time period for which this was the case. For example, Philip Hammond holding the position of Foreign Secretary between two dates."@en ;
	rdfs:isDefinedBy <http://parliament.uk/ontologies/agency/> .

pa:Position rdf:type owl:Class ;
	rdfs:label "Position"@en ;
	rdfs:comment "A named position, having existence over time, which may be held by one or more people, or have no current incumbency. For example, Minister of Food, a position having existed in the past."@en ;
	rdfs:isDefinedBy <http://parliament.uk/ontologies/agency/> .
	
pa:GroupInclusion rdf:type owl:Class ;
	rdfs:label "Group inclusion"@en ;
	rdfs:comment "The inclusion of a person or group in another group over a period of time. For example, a membership of a committee or a whipping to a party."@en ;
	rdfs:isDefinedBy <http://parliament.uk/ontologies/agency/> .
	
pa:Place rdf:type owl:Class ;
	rdfs:label "Place"@en ;
	rdfs:comment "A place named in a geography."@en ;
	rdfs:isDefinedBy <http://parliament.uk/ontologies/agency/> .
	
skos:Concept rdf:type owl:Class ;
	rdfs:label "Concept"@en ;
	rdfs:isDefinedBy <http://www.w3.org/2004/02/skos/core> .
	
				

#######  Object properties ##### 
	
pa:hasExpertiseIn rdf:type owl:ObjectProperty ;
	rdfs:label "Has expertise in"@en ;
	rdfs:comment "Relates an agent to a concept to express an area of expertise. An agent may have one or more areas of expertise, or none."@en ;
	rdfs:domain pa:Agent ;
	rdfs:range skos:Concept ;
	rdfs:isDefinedBy <http://parliament.uk/ontologies/agency/> .
	
pa:hasInterestIn rdf:type owl:ObjectProperty ;
	rdfs:label "Has interest in"@en ;
	rdfs:comment "Relates an agent to a concept to express an area of interest. An agent may have one or more areas of interest, or none."@en ;
	rdfs:domain pa:Agent ;
	rdfs:range skos:Concept ;
	rdfs:isDefinedBy <http://parliament.uk/ontologies/agency/> .
	
pa:hasGroupInclusion rdf:type owl:ObjectProperty ;
	rdfs:label "Has group inclusion"@en ;
	rdfs:comment "Relates an agent to a group inclusion. An agent may have one or more group inclusions, or none. A group inclusion is to a single agent."@en ;
	rdfs:domain pa:Agent ;
	rdfs:range pa:GroupInclusion ;
	rdfs:isDefinedBy <http://parliament.uk/ontologies/agency/> .
	
pa:hasIncumbency rdf:type owl:ObjectProperty ;
	rdfs:label "Has incumbency"@en ;
	rdfs:comment "Relates a person to an incumbency. A person may have one or more incumbencies, or none. An incumbency is to a single person."@en ;
	rdfs:domain pa:Person ;
	rdfs:range pa:Incumbency ;
	rdfs:isDefinedBy <http://parliament.uk/ontologies/agency/> .
	
pa:hasPosition rdf:type owl:ObjectProperty ;
	rdfs:label "Has position"@en ;
	rdfs:comment "Relates an incumbency to a position. An incumbency is to a single position. A position may have one or more incumbencies, or none."@en ;
	rdfs:domain pa:Incumbency ;
	rdfs:range pa:Position ;
	rdfs:isDefinedBy <http://parliament.uk/ontologies/agency/> .
	
pa:positionIn rdf:type owl:ObjectProperty ;
	rdfs:label "Position in"@en ;
	rdfs:comment "Relates a position to a group. A position is in a single group. A group may have one or more positions, or none."@en ;
	rdfs:domain pa:Position ;
	rdfs:range pa:Group ;
	rdfs:isDefinedBy <http://parliament.uk/ontologies/agency/> .				
	
pa:inGroup rdf:type owl:ObjectProperty ;
	rdfs:label "In group"@en ;
	rdfs:comment "Relates a group inclusion to a group. A group inclusion is in a single group. A group may have one or more group inclusions, or none."@en ;
	rdfs:domain pa:GroupInclusion ;
	rdfs:range pa:Group ;
	rdfs:isDefinedBy <http://parliament.uk/ontologies/agency/> .	
	
pa:placeOfBirth rdf:type owl:ObjectProperty ;
	rdfs:label "Place of birth"@en ;
	rdfs:comment "Relates a person to their place of birth."@en ;
	rdfs:domain pa:Person ;
	rdfs:range pa:Place ;
	rdfs:isDefinedBy <http://parliament.uk/ontologies/agency/> .

	
	
#######  Data properties ##### 


### To be replaced by a full time bound person name model ###
pa:title rdf:type owl:DatatypeProperty ;
	rdfs:label "Title"@en ;
	rdfs:comment "A person's title. For example, Mr., Ms. or Dr."@en ;
	rdfs:domain pa:Person ;
	rdfs:range rdf:langString ;
	rdfs:isDefinedBy <http://parliament.uk/ontologies/agency/> .	

pa:givenName rdf:type owl:DatatypeProperty ;
	rdfs:label "Given name"@en ;
	rdfs:comment "A person's personal name, commonly known in the west as first or forename."@en ;
	rdfs:domain pa:Person ;
	rdfs:range rdf:langString ;
	rdfs:isDefinedBy <http://parliament.uk/ontologies/agency/> .	

pa:otherNames rdf:type owl:DatatypeProperty ;
	rdfs:label "Other names"@en ;
	rdfs:comment "A person's additional given names."@en ;
	rdfs:domain pa:Person ;
	rdfs:range rdf:langString ;
	rdfs:isDefinedBy <http://parliament.uk/ontologies/agency/> .	

pa:familyName rdf:type owl:DatatypeProperty ;
	rdfs:label "Family name"@en ;
	rdfs:comment "A person's inherited name, commonly known in the west as surname."@en ;
	rdfs:domain pa:Person ;
	rdfs:range rdf:langString ;
	rdfs:isDefinedBy <http://parliament.uk/ontologies/agency/> .
### To be replaced by a full time bound person name model ###

pa:dateOfBirth rdf:type owl:DatatypeProperty ;
	rdfs:label "Date of birth"@en ;
	rdfs:comment "A person's date of birth."@en ;
	rdfs:domain pa:Person ;
	rdfs:range xsd:date ;
	rdfs:isDefinedBy <http://parliament.uk/ontologies/agency/> .

pa:dateOfDeath rdf:type owl:DatatypeProperty ;
	rdfs:label "Date of death"@en ;
	rdfs:comment "A person's date of death."@en ;
	rdfs:domain pa:Person ;
	rdfs:range xsd:date ;
	rdfs:isDefinedBy <http://parliament.uk/ontologies/agency/> .