@prefix pfb: <http://parliament.uk/ontologies/formal-body/> . 
@prefix xsd: <http://www.w3.org/2001/XMLSchema#> . 
@prefix rdf: <http://www.w3.org/1999/02/22-rdf-syntax-ns#> .
@prefix dcterms: <http://purl.org/dc/terms/> .
@prefix owl:     <http://www.w3.org/2002/07/owl#> .
@prefix rdfs:    <http://www.w3.org/2000/01/rdf-schema#> .
@prefix foaf:	<http://xmlns.com/foaf/0.1/> .

<http://parliament.uk/ontologies/formal-body/> 
    rdf:type owl:Ontology ;
    dcterms:title "Formal body ontology"@en ;
    dcterms:created "2017-08-29"^^xsd:date ;
	dcterms:rights "Open Parliament Licence v3.0"@en ;
    dcterms:description "An ontology to describe committees and committee like bodies."@en ;
	foaf:depiction <https://ukparliament.github.io/ontologies/formal-body/formal-body.png> ;
	foaf:maker
		[ foaf:name "James Bowman" ],
		[ foaf:name "Robert Brook"; foaf:homepage <https://robert-brook.com/> ],
		[ foaf:name "Gordon Clark" ],
		[ foaf:name "Edward McCarthy" ],
		[ foaf:name "Silver Oliver" ],
		[ foaf:name "Michael Smethurst"; foaf:homepage <http://smethur.st/> ],
	    [ foaf:name "Anya Somerville" ].


#######  Classes ##### 	

pfb:FormalBody rdf:type owl:Class ;
	rdfs:label "Formal body"@en ;
	rdfs:comment "A group of people with a specific remit engaging in the formal business of Parliament. Usually these are committees or committee-like bodies established by Parliament. Sometimes formally constituted by Parliamentary procedure (e.g. via Standing Orders), sometimes constituted on a less formal basis (e.g. the Lord Speaker's Advisory Panel on Works of Art). Some formal bodies are established outside Parliament but still have a formal link to Parliament (e.g. the Intelligence and Security Committee of Parliament). Some formal bodies are established under statute. Formal bodies usually consist of a subset of Members of Parliament from the House of Commons, or peers from the House of Lords, or a mix of both appointed to deal with particular areas or issues. Occasionally a House meets as a Committee of the Whole House allowing all members of the House to attend and participate. Formal body membership generally reflects the political makeup of the House. All Party Parliamentary Groups are informal groupings of members with no formal place in the legislature so do not fit within this category."@en ;
	rdfs:isDefinedBy <http://parliament.uk/ontologies/formal-body/> .
	
pfb:ParliamentaryCommittee rdf:type owl:Class ;
	rdfs:subClassOf pfb:FormalBody ;
	rdfs:label "Parliamentary committee"@en ;
	rdfs:comment "Parliamentary Committees are formed and appointed by one or both Houses by means of a motion or Standing Order."@en ;
	rdfs:isDefinedBy <http://parliament.uk/ontologies/formal-body/> .

pfb:SelectCommittee rdf:type owl:Class ;
	rdfs:subClassOf pfb:ParliamentaryCommittee ;
	rdfs:label "Select Committee"@en ;
	rdfs:comment "Select Committees work in both Houses. They check and report on areas ranging from the work of government departments to economic affairs. The results of these inquiries are public and many require a response from the government. House of Commons Select Committees are largely concerned with examining the work of government departments. Select Committees in the House of Lords concentrate on broader themes rather than individual departments."@en ;
	rdfs:isDefinedBy <http://parliament.uk/ontologies/formal-body/> .

pfb:GeneralCommittee rdf:type owl:Class ;
	rdfs:subClassOf pfb:ParliamentaryCommittee ;
	rdfs:label "General Committee"@en ;
	rdfs:comment "The main role of General Committees is to consider proposed legislation in detail. This committee system allows faster processing of bills and is unique to the House of Commons; the Lords meet as a whole House in this function. There are various types of General Committee: Committees on Bills, Grand Committees looking at matters specific to the devolved nations of the UK, and General Committees on delegated legislation and European documents."@en ;
	rdfs:isDefinedBy <http://parliament.uk/ontologies/formal-body/> .

pfb:NonSelectCommittee rdf:type owl:Class ;
	rdfs:subClassOf pfb:ParliamentaryCommittee ;
	rdfs:label "Non Select Committee"@en ;
	rdfs:comment "The House of Lords does not have General Committees but does have non-Select Committees. At a Select Committee of the House of Lords, Peers are not excluded from attending and speaking but they must not attend any meeting while the Committee deliberate, unless invited by the Committee to do so, and they must not vote. At a non-Select Committee, any Peer can attend, speak and vote."@en ;
	rdfs:isDefinedBy <http://parliament.uk/ontologies/formal-body/> .

pfb:StatutoryCommittee rdf:type owl:Class ;
	rdfs:subClassOf pfb:FormalBody ;
	rdfs:label "StatutoryCommittee"@en ;
	rdfs:comment "Statutory Committees are formed as a result of legislation. For example, the Ecclesiastical Committee."@en ;
	rdfs:isDefinedBy <http://parliament.uk/ontologies/formal-body/> .

pfb:InformallyConstitutedCommittee rdf:type owl:Class ;
	rdfs:subClassOf pfb:FormalBody ;
	rdfs:label "InformallyConstitutedCommittee"@en ;
	rdfs:comment "An InformallyConstitutedCommittee is a committee-like body that is not established under Parliamentary procedure or by statute."@en ;
	rdfs:isDefinedBy <http://parliament.uk/ontologies/formal-body/> .

pfb:FocusCategory rdf:type owl:Class ;
	rdfs:label "Focus category"@en ;
	rdfs:comment "Provides a way to aggregate formal bodies by the type of thing they focus on or scrutinise. In theory this could be derived from any 'focus' relationships, but in some cases the thing these classes point at are not well enough defined to determine their type. For example, the Scottish Grand Committee would point at a library subject heading / concept of Scotland. This concept is only typed as a geographic entity, and not identified as a devolved nation. Aggregating a list of formal bodies with a focus on devolved nations would not be possible from the 'focus' relationships alone. Therefore, we introduced focus category to give a higher level means to group formal bodies by interest areas. To give another example, 'focus' might point to a named item of legislation, and the focus category would say that this Formal Body was constituted to scrutinise a specific item of legislation but not identify which one. Options for focus category are: a specific item of legislation, a type of legislation, one or more government departments, matters specific to devolved nations etc."@en ;
	rdfs:isDefinedBy <http://parliament.uk/ontologies/formal-body/> .
	
pfb:House rdf:type owl:Class ;
	rdfs:label "House"@en ;
	rdfs:comment "A parliamentary House. For example, the House of Lords"@en ;
	rdfs:isDefinedBy <http://parliament.uk/ontologies/formal-body/> .
	
pfb:WorkPackage rdf:type owl:Class ;
	rdfs:label "Work package"@en ;
	rdfs:comment "A grouping of business items which may be a group falling under a procedure, or a grouping determined by a committee. For example, business items considered during the passage of a particular statutory instrument or public bill, or during an inquiry by a select committee."@en ;
	rdfs:isDefinedBy <http://parliament.uk/ontologies/formal-body/> .
	
pfb:Inquiry rdf:type owl:Class ;
	rdfs:subClassOf pfb:WorkPackage ;
	rdfs:label "Inquiry"@en ;
	rdfs:comment "A type of work package investigating a specific subject or policy area."@en ;
	rdfs:isDefinedBy <http://parliament.uk/ontologies/formal-body/> .
	
pfb:InquiryScope rdf:type owl:Class ;
	rdfs:label "Inquiry scope"@en ;
	rdfs:comment "The scope or terms of reference of an inquiry. Sets out the context, constraints and questions which the inquiry seeks to address."@en ;
	rdfs:isDefinedBy <http://parliament.uk/ontologies/formal-body/> .
	
pfb:WorkPackageType rdf:type owl:Class ;
	rdfs:label "Work package type"@en ;
	rdfs:comment "Used to describe the type of a work package. Whilst inquiries have a specific Inquiry subclass, work package type is intended to describe non-inquiry work packages. For example, a collection of hearings before a person is appointed to a public body or a set of hearings where a government minister appears before a committee."@en ;
	rdfs:isDefinedBy <http://parliament.uk/ontologies/formal-body/> .
	
pfb:BusinessItem rdf:type owl:Class ;
	rdfs:label "Business item"@en ;
	rdfs:comment "An item of business conducted either within or outside Parliament. For example: a second reading debate, the tabling of an early day motion, a laying of a paper, the making of a statutory instrument by a government minister."@en ;
	rdfs:isDefinedBy <http://parliament.uk/ontologies/formal-body/> .
	
pfb:Focus rdf:type owl:Class ;
	rdfs:label "Focus"@en ;
	rdfs:comment "A focus area for a formal body or work package. This might be a government department, a type of legislation, an item of legislation or a SKOS type concept."@en ;
	rdfs:isDefinedBy <http://parliament.uk/ontologies/formal-body/> .
	
	
	
#######  Object properties ##### 

pfb:belongsToHouse rdf:type owl:ObjectProperty ;
	rdfs:label "Belongs to house"@en ;
	rdfs:comment "Relates a formal body to the House or Houses it belongs to. A joint committee will belong to both Houses."@en ;
	rdfs:domain pfb:FormalBody ;
	rdfs:range pfb:House ;
	rdfs:isDefinedBy <http://parliament.uk/ontologies/formal-body/> .

pfb:hasLeadHouse rdf:type owl:ObjectProperty ;
	rdfs:label "Has lead house"@en ;
	rdfs:comment "A joint committee will have a lead House responsible for its administration."@en ;
	rdfs:domain pfb:FormalBody ;
	rdfs:range pfb:House ;
	rdfs:isDefinedBy <http://parliament.uk/ontologies/formal-body/> .
	
pfb:hasParentFormalBody rdf:type owl:ObjectProperty ;
	rdfs:label "Has parent formal body"@en ;
	rdfs:comment "Allows for committees to have sub-committees and sub-committees to have parent committees."@en ;
	rdfs:domain pfb:FormalBody ;
	rdfs:range pfb:FormalBody ;
	rdfs:isDefinedBy <http://parliament.uk/ontologies/formal-body/> .
	
pfb:undertakesWorkPackage rdf:type owl:ObjectProperty ;
	rdfs:label "Undertakes work package"@en ;
	rdfs:comment "Allows for formal bodies to take on work packages like inquiries. A joint inquiry will have more than one associated formal body."@en ;
	rdfs:domain pfb:FormalBody ;
	rdfs:range pfb:WorkPackage ;
	rdfs:isDefinedBy <http://parliament.uk/ontologies/formal-body/> .

pfb:hasParentWorkPackage rdf:type owl:ObjectProperty ;
	rdfs:label "Has parent work package"@en ;
	rdfs:comment "Allows for work packages to have parent work packages. e.g. a sub-inquiry can belong to a wider inquiry."@en ;
	rdfs:domain pfb:WorkPackage ;
	rdfs:range pfb:WorkPackage ;
	rdfs:isDefinedBy <http://parliament.uk/ontologies/formal-body/> .
	
pfb:hasInquiryScope rdf:type owl:ObjectProperty ;
	rdfs:label "Has inquiry scope"@en ;
	rdfs:comment "Relates an inquiry to its scope or terms of reference."@en ;
	rdfs:domain pfb:Inquiry ;
	rdfs:range pfb:InquiryScope ;
	rdfs:isDefinedBy <http://parliament.uk/ontologies/formal-body/> .
	
pfb:hasWorkPackageType rdf:type owl:ObjectProperty ;
	rdfs:label "Has work package type"@en ;
	rdfs:comment "Defines the type of a work package where the work package is not an inquiry."@en ;
	rdfs:domain pfb:WorkPackage ;
	rdfs:range pfb:WorkPackageType ;
	rdfs:isDefinedBy <http://parliament.uk/ontologies/formal-body/> .
	
pfb:formsPartOf rdf:type owl:ObjectProperty ;
	rdfs:label "Forms part of"@en ;
	rdfs:comment "Relates a business item to a work package it forms part of. One or more business items may form part of a work package. A business item may form part of one or more work packages. For example, a meeting of the Joint Committee on Statutory Instruments may consider one or more SIs, each SI being the focus of a separate work package."@en ;
	rdfs:domain pfb:BusinessItem ;
	rdfs:range pfb:WorkPackage ;
	rdfs:isDefinedBy <http://parliament.uk/ontologies/formal-body/> .
	
pfb:hasAgent rdf:type owl:ObjectProperty ;
	rdfs:label "Has agent"@en ;
	rdfs:comment "Associates a business item with the formal body responsible for organising it. A business item may be run by more than one formal body. For example, a joint evidence session."@en ;
	rdfs:domain pfb:BusinessItem ;
	rdfs:range pfb:FormalBody ;
	rdfs:isDefinedBy <http://parliament.uk/ontologies/formal-body/> .
	
pfb:formalBodyFocus rdf:type owl:ObjectProperty ;
	rdfs:label "Formal body focus"@en ;
	rdfs:comment "Associates a formal body with its area of focus."@en ;
	rdfs:domain pfb:FormalBody ;
	rdfs:range pfb:Focus ;
	rdfs:isDefinedBy <http://parliament.uk/ontologies/formal-body/> .

pfb:workPackageFocus rdf:type owl:ObjectProperty ;
	rdfs:label "Work package focus"@en ;
	rdfs:comment "Associates a work package with its area of focus."@en ;
	rdfs:domain pfb:WorkPackage ;
	rdfs:range pfb:Focus ;
	rdfs:isDefinedBy <http://parliament.uk/ontologies/formal-body/> .

pfb:hasFocusCategory rdf:type owl:ObjectProperty ;
	rdfs:label "hasFocusCategory"@en ;
	rdfs:comment "Relates a formal body to its focus category."@en ;
	rdfs:domain pfb:FormalBody ;
	rdfs:range pfb:FocusCategory ;
	rdfs:isDefinedBy <http://parliament.uk/ontologies/formal-body/> .
				

#######  Data properties ##### 

pfb:remit rdf:type owl:DatatypeProperty ;
	rdfs:label "remit"@en ;
	rdfs:comment "The task or area of activity officially assigned to a formal body. This is a textual description as opposed to Focus which points at entities to describe the areas to be examined."@en ;
	rdfs:domain pfb:FormalBody ;
	rdfs:range rdf:langString ;
	rdfs:isDefinedBy <http://parliament.uk/ontologies/formal-body/> .