@prefix pfba: <http://parliament.uk/ontologies/formal-body-affiliation/> . 
@prefix xsd: <http://www.w3.org/2001/XMLSchema#> . 
@prefix rdf: <http://www.w3.org/1999/02/22-rdf-syntax-ns#> .
@prefix dcterms: <http://purl.org/dc/terms/> .
@prefix owl:     <http://www.w3.org/2002/07/owl#> .
@prefix rdfs:    <http://www.w3.org/2000/01/rdf-schema#> .
@prefix foaf:	<http://xmlns.com/foaf/0.1/> .

<http://parliament.uk/ontologies/formal-body-affiliation/> 
    rdf:type owl:Ontology ;
    dcterms:title "Formal body affiliation ontology"@en ;
    dcterms:created "2017-06-22"^^xsd:date ;
	dcterms:rights "Open Parliament Licence v3.0"@en ;
    dcterms:description "An ontology to extend the agency model to specialise group inclusion and position to formal bodies."@en ;
	foaf:depiction <https://ukparliament.github.io/ontologies/formal-body-affiliation/formal-body-affiliation.png> ;
	foaf:maker
		[ foaf:name "Robert Brook"; foaf:homepage <https://robert-brook.com/> ],
		[ foaf:name "Edward McCarthy" ],
		[ foaf:name "Silver Oliver" ],
		[ foaf:name "Michael Smethurst"; foaf:homepage <http://smethur.st/> ],
	    [ foaf:name "Anya Somerville" ].


#######  Classes ##### 	

pfba:GroupInclusion rdf:type owl:Class ;
	rdfs:label "Group inclusion"@en ;
	rdfs:comment "The inclusion of a person or group in another group over a period of time. For example, a membership of a committee or a whipping to a party."@en ;
	rdfs:isDefinedBy <http://parliament.uk/ontologies/formal-body-affiliation/> .
	
pfba:FormalBodyMembership rdf:type owl:Class ;
	rdfs:subClassOf pfba:GroupInclusion ;
	rdfs:label "Formal body membership"@en ;
	rdfs:comment "Specialises group inclusion to membership of a formal body - a committee-like groups. In most cases membership is drawn from the backbenches of a House. Occasionally people who are subject area experts but not Members of either House will appointed as members of a committee. Usually membership will be assigned by one of the two Houses. Co-opted members are appointed by the existing members of a committee."@en ;
	rdfs:isDefinedBy <http://parliament.uk/ontologies/formal-body-affiliation/> .
	
pfba:CooptedMembership rdf:type owl:Class ;
	rdfs:subClassOf pfba:FormalBodyMembership ;
	rdfs:label "Coopted membership"@en ;
	rdfs:comment "A member of a committee who is invited to join on occasion. Co-opted members might be drawn from people who are not Members of a House. These are referred to as lay members in the House of Commons and external members in the House of Lords For example, the Executive Committee will occasionally co-opt the Director of the Parliamentary Digital Service and / or Parliamentary Security Director into its membership. Sometimes a co-opted member will be drawn from the membership of a House e.g. in the House of Lords a peer who is a subject matter expert might be co-opted onto a committee."@en ;
	rdfs:isDefinedBy <http://parliament.uk/ontologies/formal-body-affiliation/> .
	
pfba:AlternateMembership rdf:type owl:Class ;
	rdfs:subClassOf pfba:FormalBodyMembership ;
	rdfs:label "Alternate membership"@en ;
	rdfs:comment "Alternate members act as substitutes when other members are unable to attend. For example, the Lords Procedure Committee is supplemented by one alternate for each party group of backbench members and one for the Crossbenchers, plus an alternate for the Convenor. They receive papers and if any of the relevant members cannot attend, alternate members are entitled to attend and vote."@en ;
	rdfs:isDefinedBy <http://parliament.uk/ontologies/formal-body-affiliation/> .
	
pfba:ExOfficioMembership rdf:type owl:Class ;
	rdfs:subClassOf pfba:FormalBodyMembership ;
	rdfs:label "Ex-officio membership"@en ;
	rdfs:comment "Ex-officios are members appointed by virtue of roles or positions, by convention. Some Ministers are appointed ex-officio members of committees. Examples include Government and Opposition Whips regularly serving on the Administration Committee; specific government Ministers being members of (but by convention not attending meetings of) the Committee of Public Accounts and the Environmental Audit Committee; and successive Leaders of the House chairing the Select Committee on Modernisation of the House of Commons between 1997 and 2010."@en ;
	rdfs:isDefinedBy <http://parliament.uk/ontologies/formal-body-affiliation/> .
	
pfba:Position rdf:type owl:Class ;
	rdfs:label "Position"@en ;
	rdfs:comment "A named position, having existence over time, which may be held by one or more people, or have no current incumbency. For example, Minister of Food, a position having existed in the past."@en ;
	rdfs:isDefinedBy <http://parliament.uk/ontologies/formal-body-affiliation/> .
	
pfba:FormalBodyPosition rdf:type owl:Class ;
	rdfs:subClassOf pfba:Position ;
	rdfs:label "Formal body position"@en ;
	rdfs:comment "Specialises position to formal bodies."@en ;
	rdfs:isDefinedBy <http://parliament.uk/ontologies/formal-body-affiliation/> .
	
pfba:Chair rdf:type owl:Class ;
	rdfs:subClassOf pfba:FormalBodyPosition ;
	rdfs:label "Chair"@en ;
	rdfs:comment "Used to describe the position of chair of a formal body. A formal body may have more that one incumbency in the chair position at the same time, or none."@en ;
	rdfs:isDefinedBy <http://parliament.uk/ontologies/formal-body-affiliation/> .
	
pfba:CommitteeClerk rdf:type owl:Class ;
	rdfs:subClassOf pfba:FormalBodyPosition ;
	rdfs:label "Committee clerk"@en ;
	rdfs:comment "Used to describe the principal clerk of a formal body."@en ;
	rdfs:isDefinedBy <http://parliament.uk/ontologies/formal-body-affiliation/> .
	
pfba:InternalExpert rdf:type owl:Class ;
	rdfs:subClassOf pfba:FormalBodyPosition ;
	rdfs:label "Internal expert"@en ;
	rdfs:comment "Formal bodies are able to appoint subject matter experts. The role is normally described as committee specialist within Parliament."@en ;
	rdfs:isDefinedBy <http://parliament.uk/ontologies/formal-body-affiliation/> .
	
pfba:ExternalExpert rdf:type owl:Class ;
	rdfs:subClassOf pfba:FormalBodyPosition ;
	rdfs:label "External expert"@en ;
	rdfs:comment "Formal bodies can contract subject matter experts for the duration of an inquiry."@en ;
	rdfs:isDefinedBy <http://parliament.uk/ontologies/formal-body-affiliation/> .