@prefix ppr: <http://parliament.uk/ontologies/procedure/> . 
@prefix xsd: <http://www.w3.org/2001/XMLSchema#> . 
@prefix rdf: <http://www.w3.org/1999/02/22-rdf-syntax-ns#> .
@prefix dcterms: <http://purl.org/dc/terms/> .
@prefix owl:     <http://www.w3.org/2002/07/owl#> .
@prefix rdfs:    <http://www.w3.org/2000/01/rdf-schema#> .
@prefix foaf:	<http://xmlns.com/foaf/0.1/> .

<http://parliament.uk/ontologies/procedure/> 
    rdf:type owl:Ontology ;
    dcterms:title "Procedure ontology"@en ;
    dcterms:created "2018-02-20"^^xsd:date ;
	dcterms:rights "Open Parliament Licence v3.0"@en ;
    dcterms:description "Procedure ontology for UK Parliament. An abstract ontology for describing how process steps or stages can be combined into a procedure. In this model, the procedure is analogous to a journey map to a set of potential destinations, a route is a set of directions on one of those journeys and a step is a waypoint."@en ;
	foaf:depiction <https://ukparliament.github.io/ontologies/procedure/procedure.png> ;
	foaf:maker
		[ foaf:name "David Beamish" ],
		[ foaf:name "Robert Brook"; foaf:homepage <https://robert-brook.com/> ],
		[ foaf:name "Gordon Clarke" ],
		[ foaf:name "Jack Dent" ],
		[ foaf:name "Samu Lang" ],
		[ foaf:name "Silver Oliver" ],
		[ foaf:name "Michael Smethurst"; foaf:homepage <http://smethur.st/> ],
	    [ foaf:name "Anya Somerville" ],
		[ foaf:name "James Vintner" ],
		[ foaf:name "Jane White" ],
		[ foaf:name "Ben Woodhams" ].


#######  Classes #####
	
ppr:Procedure rdf:type owl:Class ;
	rdfs:label "Procedure"@en ;
	rdfs:comment "A procedure in a House or Houses. For example, the passage of a made affirmative statutory instrument in both Houses. A procedure may consist of business in a particular House, such as a division; business undertaken by both Houses jointly, such as a joint committee; processes applying to either House, such as a time period; and activities outside Parliament, such as the making of a statutory instrument. In this model a procedure that consists of business in both Houses is considered as a single procedure."@en ;
	rdfs:isDefinedBy <http://parliament.uk/ontologies/procedure/> .
	
ppr:Route rdf:type owl:Class ;
	rdfs:label "Route"@en ;
	rdfs:comment "A route is a link from one step or logic gate to one step or logic gate. A route source may also be its destination. A route is available only when the input step is True, actualised by a business item having a date in the past, or by the input from a logic gate operation being True. Where a route has a start or end date it indicates the validity period for that route."@en ;
	rdfs:isDefinedBy <http://parliament.uk/ontologies/procedure/> .
	
ppr:RouteType rdf:type owl:Class ;
	rdfs:label "Route type"@en ;
	rdfs:comment "A route type is one of causes, allows, requires and precludes. A route with type 'causes' relates a preceding step (linked via fromStep) to a following step (linked via toStep) where actualisation of the preceding step by a business item with a date in the past causes the inevitability of the following step. A route with type 'allows' relates a preceding step to a following step where actualisation of the preceding step by a business item with a date in the past allows but does not cause the following step. A route with type 'requires' relates a preceding step to a following step where actualisation of the following step by a business item with a date in the past is necessary before the preceding step can happen. A route with type 'precludes' relates a preceding step to a following step where actualisation of the preceding step by a business item with a date in the past precludes the following step. Particular steps occur only once in a work package. For example, in the made affirmative statutory instrument procedure the step 'cleared by the Joint Committee on Statutory Instruments' may happen only once. A route with the type 'precludes' may route a step to the same step. When a step is actualised by a business item with a date in the past, further instances of that step being actualised in the work package become precluded."@en ;
	rdfs:isDefinedBy <http://parliament.uk/ontologies/procedure/> .

ppr:LogicGate rdf:type owl:Class ;
	rdfs:label "Logic gate"@en ;
	rdfs:comment "A logic gate routes from a step or a logic gate and routes to a step or a logic gate. A gate performs one logical operation on one or more routes. Both the input and the output of a logic gate are either true or false."@en ;
	rdfs:isDefinedBy <http://parliament.uk/ontologies/procedure/> .
	
ppr:LogicGateType rdf:type owl:Class ;
	rdfs:label "Logic gate type"@en ;
	rdfs:comment "A logic gate has a type of NOT, AND or OR. A logic gate with type NOT when given True has the result False and when given False has the result True. A logic gate with type AND takes at least two routes as inputs: if all are True the output route is True. A logic gate with type OR takes at least two routes as inputs: if at least one is True the output route is True."@en ;
	rdfs:isDefinedBy <http://parliament.uk/ontologies/procedure/> .
	
ppr:Step rdf:type owl:Class ;
	rdfs:label "Step"@en ;
	rdfs:comment "A step forming part of a procedure by means of a route. For example, English Votes for English Laws (EVEL) consideration of a  a statutory instrument. Steps may form part of more than one procedure. For example, all statutory instruments are subject to EVEL consideration."@en ;
	rdfs:isDefinedBy <http://parliament.uk/ontologies/procedure/> .
	
ppr:House rdf:type owl:Class ;
	rdfs:label "House"@en ;
	rdfs:comment "A House forming part of a parliament. For example, the House of Lords."@en ;
	rdfs:isDefinedBy <http://parliament.uk/ontologies/procedure/> .
	
ppr:BusinessItem rdf:type owl:Class ;
	rdfs:label "Business item"@en ;
	rdfs:comment "An item of business conducted either within Parliament or outside Parliament and producing an outcome subject to procedure. For example: a second reading debate, the tabling of an early day motion, a laying of a paper, the making of a statutory instrument by a government minister."@en ;
	rdfs:isDefinedBy <http://parliament.uk/ontologies/procedure/> .
	
ppr:WorkPackage rdf:type owl:Class ;
	rdfs:label "Work package"@en ;
	rdfs:comment "A grouping of business items being considered together. Membership of a work package group is constrained by the capacity of a business item to actualise a step in the applicable procedure. For example, business items during the passage of a particular statutory instrument, or during the passage of a particular public bill."@en ;
	rdfs:isDefinedBy <http://parliament.uk/ontologies/procedure/> .
	
ppr:WorkPackageableThing rdf:type owl:Class ;
	rdfs:label "Work packageable thing"@en ;
	rdfs:comment "A thing resulting in business items grouped into a work package. The model describes the relationship between a work package and a workpackageable thing as the focus of the work package."@en ;
	rdfs:isDefinedBy <http://parliament.uk/ontologies/procedure/> .
	
	
	
#######  Object properties ##### 

ppr:formsPartOf rdf:type owl:ObjectProperty ;
	rdfs:label "Forms part of"@en ;
	rdfs:comment "Relates a particular business item to the work package it forms part of. A work package may be formed of more than one business item and a particular business item may be included in more than one work package. For example, a meeting of the Joint Committee on Statutory Instruments may consider one or more SIs, with each SI being the focus of a separate work package."@en ;
	rdfs:domain ppr:BusinessItem ;
	rdfs:range ppr:WorkPackage ;
	rdfs:isDefinedBy <http://parliament.uk/ontologies/procedure/> .
	
ppr:subjectTo rdf:type owl:ObjectProperty ;
	rdfs:label "Subject to"@en ;
	rdfs:comment "Relates a work packageable thing to the procedure it is subject to. A work packageable thing is only subject to one procedure."@en ;
	rdfs:domain ppr:WorkPackageableThing ;
	rdfs:range ppr:Procedure ;
	rdfs:isDefinedBy <http://parliament.uk/ontologies/procedure/> .
	
ppr:actualises rdf:type owl:ObjectProperty ;
	rdfs:label "Actualises"@en ;
	rdfs:comment "Relates a business item to a step in a procedure via a route. For example, relating the second reading of a public bill to the second reading step in the procedure. Whilst a step may be actualised by more than one business item in different work packages, a business item may actualise one or more steps. For example, a business item appearing in the Order Paper including a debate on several motions may actualise steps relating to each motion."@en ;
	rdfs:domain ppr:BusinessItem ;
	rdfs:range ppr:Step ;
	rdfs:isDefinedBy <http://parliament.uk/ontologies/procedure/> .

ppr:fromStep rdf:type owl:ObjectProperty ;
	rdfs:label "From step"@en ;
	rdfs:comment "Relates a route to its input step."@en ;
	rdfs:domain ppr:Route ;
	rdfs:range ppr:Step ;
	rdfs:isDefinedBy <http://parliament.uk/ontologies/procedure/> .
	
ppr:toStep rdf:type owl:ObjectProperty ;
	rdfs:label "To step"@en ;
	rdfs:comment "Relates a route to its output step."@en ;
	rdfs:domain ppr:Route ;
	rdfs:range ppr:Step ;
	rdfs:isDefinedBy <http://parliament.uk/ontologies/procedure/> .
	
ppr:hasRouteType rdf:type owl:ObjectProperty ;
	rdfs:label "Has route type"@en ;
	rdfs:comment "Relates a route to a route type. A route has one type."@en ;
	rdfs:domain ppr:Route ;
	rdfs:range ppr:RouteType ;
	rdfs:isDefinedBy <http://parliament.uk/ontologies/procedure/> .
	
ppr:fromLogicGate rdf:type owl:ObjectProperty ;
	rdfs:label "From logic gate"@en ;
	rdfs:comment "Relates a route to its input logic gate."@en ;
	rdfs:domain ppr:Route ;
	rdfs:range ppr:LogicGate ;
	rdfs:isDefinedBy <http://parliament.uk/ontologies/procedure/> .
	
ppr:toLogicGate rdf:type owl:ObjectProperty ;
	rdfs:label "To logic gate"@en ;
	rdfs:comment "Relates a route to its output logic gate."@en ;
	rdfs:domain ppr:Route ;
	rdfs:range ppr:LogicGate ;
	rdfs:isDefinedBy <http://parliament.uk/ontologies/procedure/> .
	
ppr:hasLogicGateType rdf:type owl:ObjectProperty ;
	rdfs:label "Has logic gate type"@en ;
	rdfs:comment "Relates a logic gate to a logic gate type. A logic gate has one type."@en ;
	rdfs:domain ppr:LogicGate ;
	rdfs:range ppr:LogicGateType ;
	rdfs:isDefinedBy <http://parliament.uk/ontologies/procedure/> .
	
ppr:follows rdf:type owl:ObjectProperty ;
	rdfs:label "Follows"@en ;
	rdfs:comment "Relates a procedure to a route. A route forms part of one procedure."@en ;
	rdfs:domain ppr:Procedure ;
	rdfs:range ppr:Route ;
	rdfs:isDefinedBy <http://parliament.uk/ontologies/procedure/> .
	
ppr:stepInHouse rdf:type owl:ObjectProperty ;
	rdfs:label "Step in House"@en ;
	rdfs:comment "Relates a step to one or both Houses where such a relationship exists."@en ;
	rdfs:domain ppr:Step ;
	rdfs:range ppr:House ;
	rdfs:isDefinedBy <http://parliament.uk/ontologies/procedure/> .
		
ppr:procedureInHouse rdf:type owl:ObjectProperty ;
	rdfs:label "Procedure in House"@en ;
	rdfs:comment "Relates a procedure to one or both Houses."@en ;
	rdfs:domain ppr:Procedure ;
	rdfs:range ppr:House ;
	rdfs:isDefinedBy <http://parliament.uk/ontologies/procedure/> .
		
ppr:focus rdf:type owl:ObjectProperty ;
	rdfs:label "Focus"@en ;
	rdfs:comment "Relates a work package to its focus, this being a work packageable thing."@en ;
	rdfs:domain ppr:WorkPackage ;
	rdfs:range ppr:WorkPackageableThing ;
	rdfs:isDefinedBy <http://parliament.uk/ontologies/procedure/> .
